Some of Server__apply() proof

src/program_proof/mpaxos/marshal_proof.v
@@ -52,6 +52,50 @@ Admitted.
 End applyAsFollowerArgs.
 End applyAsFollowerArgs.
 
+Module applyAsFollowerReply.
+Section applyAsFollowerReply.
+Context `{!heapGS Σ}.
+
+Record C :=
+mkC {
+  err: u64 ;
+}.
+
+Definition has_encoding (encoded:list u8) (reply:C) : Prop :=
+  encoded = (u64_le reply.(err)).
+
+Context `{!heapGS Σ}.
+
+Definition own reply_ptr reply q : iProp Σ :=
+  "Hreply_err" ∷ reply_ptr ↦[mpaxos.applyAsFollowerReply :: "err"]{q} #reply.(err)
+  .
+
+Lemma wp_Encode (reply_ptr:loc) (reply:C) q :
+  {{{
+        own reply_ptr reply q
+  }}}
+    mpaxos.encodeApplyAsFollowerReply #reply_ptr
+  {{{
+        enc enc_sl, RET (slice_val enc_sl);
+        ⌜has_encoding enc reply⌝ ∗
+        is_slice enc_sl byteT 1 enc
+  }}}.
+Admitted.
+
+Lemma wp_Decode enc enc_sl (reply:C) :
+  {{{
+        ⌜has_encoding enc reply⌝ ∗
+        is_slice enc_sl byteT 1 enc
+  }}}
+    mpaxos.decodeApplyAsFollowerReply (slice_val enc_sl)
+  {{{
+        reply_ptr, RET #reply_ptr; own reply_ptr reply 1
+  }}}.
+Admitted.
+
+End applyAsFollowerReply.
+End applyAsFollowerReply.
+
 Module applyReply.
 Section applyReply.
 Context `{!heapGS Σ}.
@@ -69,16 +113,16 @@ Context `{!heapGS Σ}.
 
 Definition own args_ptr args q : iProp Σ :=
   ∃ ret_sl,
-  "Hargs_epoch" ∷ args_ptr ↦[mpaxos.applyReply :: "err"]{q} #args.(err) ∗
-  "Hargs_ret" ∷ args_ptr ↦[mpaxos.applyReply :: "ret"]{q} (slice_val ret_sl) ∗
-  "Hargs_ret_sl" ∷ is_slice_small ret_sl byteT q args.(ret)
+  "Hreply_epoch" ∷ args_ptr ↦[mpaxos.applyReply :: "err"]{q} #args.(err) ∗
+  "Hreply_ret" ∷ args_ptr ↦[mpaxos.applyReply :: "ret"]{q} (slice_val ret_sl) ∗
+  "Hreply_ret_sl" ∷ is_slice_small ret_sl byteT q args.(ret)
   .
 
 Lemma wp_Encode (args_ptr:loc) (args:C) q :
   {{{
         own args_ptr args q
   }}}
-    mpaxos.encodeApplyAsFollowerArgs #args_ptr
+    mpaxos.encodeApplyReply #args_ptr
   {{{
         enc enc_sl, RET (slice_val enc_sl);
         ⌜has_encoding enc args⌝ ∗
@@ -91,7 +135,7 @@ Lemma wp_Decode enc enc_sl (args:C) :
         ⌜has_encoding enc args⌝ ∗
         is_slice enc_sl byteT 1 enc
   }}}
-    mpaxos.decodeApplyAsFollowerArgs (slice_val enc_sl)
+    mpaxos.decodeApplyReply (slice_val enc_sl)
   {{{
         args_ptr, RET #args_ptr; own args_ptr args 1
   }}}.
